sepref correctness lemma borda

theories/Compositional_Structures/Basic_Modules/Component_Types/Electoral_Module_Ref.thy
@@ -10,7 +10,8 @@ begin
 type_synonym 'a Electoral_Module_Ref = "'a set \<Rightarrow> 'a Profile_List \<Rightarrow> 'a Result nres"
 
 abbreviation elec_mod_relb :: "('a Electoral_Module_Ref \<times> ('a set \<Rightarrow> 'a Profile \<Rightarrow> 'a Result nres)) set" where
-  "elec_mod_relb \<equiv> \<langle>Id\<rangle>alt_set_rel \<rightarrow> profile_rel \<rightarrow> \<langle>Id\<rangle>nres_rel"
+  "elec_mod_relb \<equiv> \<langle>Id\<rangle>alt_set_rel \<rightarrow> profile_rel 
+  \<rightarrow> \<langle>\<langle>Id\<rangle>set_rel \<times>\<^sub>r \<langle>Id\<rangle>set_rel \<times>\<^sub>r \<langle>Id\<rangle>set_rel\<rangle>nres_rel"
 
 definition em_rel :: "('a Electoral_Module_Ref \<times> 'a Electoral_Module) set" 
   where em_rel_def:
